FSets_Alternatives.thy
@@ -5,47 +5,57 @@ begin
 (* Alternative descriptions of finite sets and the transport of the
 recursors to the type of sets *)
 
-(* As initial semi-lattice with unit (ACIU): *)
-nonfreedata 'a fsetS = SEmp | SSingl 'a | SUn "'a fsetS" "'a fsetS"
+
+section{* As initial semi-lattice with unit (ACIU): *}
+
+nonfreedata 'a fsetS = SEmp | SSingl 'a | SUni "'a fsetS" "'a fsetS"
 where
-  Assoc: "SUn (SUn A1 A2) A3 = SUn A1 (SUn A2 A3)"
-| Comm: "SUn A1 A2 = SUn A2 A1"
-| Idem: "SUn A A = A"
-| Id: "SUn A SEmp = A"
+  Assoc: "SUni (SUni A1 A2) A3 = SUni A1 (SUni A2 A3)"
+| Comm: "SUni A1 A2 = SUni A2 A1"
+| Idem: "SUni A A = A"
+| Id: "SUni SEmp A = A"
 
-nonfreeiter asSetS :: "'a fsetS \<Rightarrow> 'a set"
+declare Idem[simp]  declare Id[simp]
+
+lemma SUni_EEp[simp]: "SUni A SEmp = A"
+by (metis Comm Id)
+
+nonfreeiter asFset :: "'a fsetS \<Rightarrow> 'a fset"
 where
-  "asSetS SEmp = {}"
-| "asSetS (SSingl a) = {a}"
-| "asSetS (SUn A1 A2) = asSetS A1 \<union> asSetS A2"
-by auto
+  "asFset SEmp = Emp"
+| "asFset (SSingl a) = Singl a"
+| "asFset (SUni A1 A2) = Uni (asFset A1) (asFset A2)"
+apply auto using Uni_assoc Uni_com by metis+
 
-lemma finite_asSetS: "finite (asSetS A)"
-by (induction rule: fsetS_induct) auto
+nonfreeiter asFsetS :: "'a fset \<Rightarrow> 'a fsetS"
+where
+  "asFsetS Emp = SEmp"
+| "asFsetS (Ins a A) = SUni (SSingl a) (asFsetS A)"
+by (metis Assoc Idem Comm)+
 
-lemma insert_asSetsS: "insert a (asSetS S) = asSetS (SUn S (SSingl a))" by auto
+lemma asFset_asFsetS[simp]: "asFset (asFsetS A) = A"
+by (induct A) (auto simp: Singl_def)
 
-lemma finite_imp_asSetS: "finite A \<Longrightarrow> (\<exists> F. A = asSetS F)"
-by (induction rule: finite_induct) (metis asSetS.simps insert_asSetsS)+
+lemma asFSetsS_Uni[simp]: "asFsetS (Uni A B) = SUni (asFsetS A) (asFsetS B)"
+apply(induction A) apply auto using Assoc
+apply metis done
 
-(*  *)
+lemma asFsetS_asFset[simp]: "asFsetS (asFset A) = A"
+apply(induction A) by (auto simp: Singl_def)
 
-term iter_fsetS
-term iter_fset
-
-
-
-
-
-term
+(* TODO:
+1) Fix associativity of Uni: the other way around.
+2) Transport to finite sets the lattice recursor.
+3) Do the same for nonempty finite sets below, without going through asSetN *)
 
 (* Nonempty finite sets, as initial semilattice (ACI): *)
-nonfreedata 'a fsetN = NSingl 'a | NUn "'a fsetN" "'a fsetN"
+nonfreedata 'a fsetN = NSingl 'a | NUni "'a fsetN" "'a fsetN"
 where
-  AssocN: "NUn (NUn A1 A2) A3 = NUn A1 (NUn A2 A3)"
-| CommN: "NUn A1 A2 = NUn A2 A1"
-| IdemN: "NUn A A = A"
+  AssocN: "NUni (NUni A1 A2) A3 = NUni A1 (NUni A2 A3)"
+| CommN: "NUni A1 A2 = NUni A2 A1"
+| IdemN: "NUni A A = A"
 
+(*
 nonfreeiter asSetN :: "'a fsetN \<Rightarrow> 'a set"
 where
   "asSetN (NSingl a) = {a}"
@@ -62,6 +72,7 @@ lemma insert_asSetsN: "insert a (asSetN S) = asSetN (NUn S (NSingl a))" by auto
 
 lemma finite_imp_asSetN: "\<lbrakk>finite A; A \<noteq> {}\<rbrakk> \<Longrightarrow> (\<exists> F. A = asSetN F)"
 by (induction rule: finite_induct) (metis asSetN.simps insert_asSetsN)+
+*)
 
 
 end
